{"cells":[{"cell_type":"markdown","source":["# Wave equation using finite difference\n\n","## Problem statement\n\n","We aim to solve the acoustic wave equation in a homogeneous rectangular\n","medium using FDTD. Mathematically, the problem is stated as follows:\n","\n$$\n\\begin{cases}\n\\begin{align}\n\\partial_t^2 u(x,y,t) - c^2 \\Delta_{xy} u(x,y,t) &= s(x,y,t) \\quad (x,y) \\in [0,L]\\times[0,H], \\quad t \\in [0,T] \\\\\nu(x,y,0) &= f(x,y) \\\\\n\\partial_t u(x,y,0) &= g(x,y) \\\\\n\\partial_n u(x,y,t) &= k(x,y,t) \\quad (x,y) \\in \\partial\\Omega, \\quad t \\in [0,T]\n\\end{align}\n\\end{cases}\n$$\n","* **Equation&#8217;s parameters are**\\\n\n","## Semi-discretization in space\n\n","We use a finite difference scheme to discretize the Laplacian operator\n","in space. Let&#8217;s introduce a uniform grid defined by its vertices of\n","coordinates :\n","\n$$\nx_i = i \\Delta x, \\quad y_j = j \\Delta y, \\quad t^n = n \\Delta t, \\quad \\text{with } i \\in [\\![0;I]\\!] \\quad \\text{and} \\quad j \\in [\\![0;J]\\!]\n$$\n","where $\\Delta x = \\frac{L}{I}$ and $\\Delta y = \\frac{H}{J}$ are the space\n","steps, and $\\Delta t$ is the time step. We denote by $u_{i,j}(t)$\n","the approximation of $u(x_i,y_j,t)$ and by $u_{i,j}^n$ the approximation\n","of $u(x_i,y_j,t^n)$.\n","\n","![ROOT:grid wave equation fdtd](ROOT:grid-wave-equation-fdtd.png)\n","\n","Inside the domain, we approximate the second-order partial derivatives\n","using three-point central differences. At the edges, except at the\n","corners, we approximate the first-order partial derivatives using\n","two-point central differences of second order. For simplicity, at the\n","corners, we approximate the first-order partial derivatives using\n","two-point off-centered differences of first order.\n","To get $u_{i,j}$ as vector, we define $U_n = u_{i,j}$ with the bijection\n","$n = n(i,j) = i+j(I+1)$. So after discretization, we write all the\n","discretized equations in the form of a linear system of the form\n","$A \\tilde U = F$, where\n","\n","- $A$ is a matrix with size $[(I+1)(J+1)]^2$,\n","- $\\tilde U = (U_1, U_2, \\ldots )$ is the vector of unknowns with size $(I+1)(J+1)$ and\n","- $F$ is the right hand side vector with size $(I+1)(J+1)$.\n","\n","## Inside the domain\n\n","Inside the domain, indices $i$ and $j$ vary in $[\\![1;I-1]\\!]$ and $[\\![1;J-1]\\!]$ respectively.\n","By expanding and summing, the discretization can be written as :\n","\n$$\nu''_{i,j}(t) - \\frac{c^2}{\\Delta y^2} u_{i,j-1}(t) - \\frac{c^2}{\\Delta x^2} u_{i-1,j}(t) + 2c^2 (\\frac{1}{\\Delta x^2} + \\frac{1}{\\Delta y^2}) u_{i,j}(t) - \\frac{c^2}{\\Delta x^2} u_{i+1,j}(t) - \\frac{c^2}{\\Delta y^2} u_{i,j+1}(t) = s_{i,j}(t)\n$$\n","which is equivalent to :\n","\n$$\nU''_n(t) - \\frac{c^2}{\\Delta y^2} U_{n-I-1}(t) - \\frac{c^2}{\\Delta x^2} U_{n-1}(t) + 2c^2 (\\frac{1}{\\Delta x^2} + \\frac{1}{\\Delta y^2}) U_n(t) - \\frac{c^2}{\\Delta x^2} U_{n+1}(t) - \\frac{c^2}{\\Delta y^2} U_{n+I+1}(t) = S_n(t)\n$$\n","where $S_n(t) = s_{i,j}(t)$.\n","We deduce the matrix $A$ and the vector $F$ as follows:\n","\n$$\n\\begin{cases}\n\\begin{align}\nA_{n,n-I-1} &= A_{n,n+I+1} = -\\frac{c^2}{\\Delta y^2} \\\\\nA_{n,n-1} &= A_{n,n+1} = -\\frac{c^2}{\\Delta x^2} \\\\\nA_{n,n} &= 2c^2 (\\frac{1}{\\Delta x^2} + \\frac{1}{\\Delta y^2}) \\\\\nF_n(t) &= S_n(t)\n\\end{align}\n\\end{cases}\n$$\n","## At the edges (except corners)\n\n","In order to approximate first-order partial derivatives using\n","two-point central differences of second order, we use the\n","virtual points located outside the domain. After that, we\n","eliminate them, so that they do not appear in the linear system.\n","## At bottom edge\n\n","At the bottom edge, indices $i$ vary in $[\\![1;I-1]\\!]$ and $j=0$.\n","By expanding and summing, the discretization can be written as :\n","\n$$\nu''_{i,0}(t) - \\frac{c^2}{\\Delta x^2} u_{i-1,0}(t) + 2c^2(\\frac{1}{\\Delta x^2} + \\frac{1}{\\Delta y^2} u_{i,0})(t) - \\frac{c^2}{\\Delta x^2} u_{i+1,0}(t) - \\frac{2c^2}{\\Delta y^2} u_{i,1}(t) = s_{i,0}(t) + \\frac{2c^2}{\\Delta y} k_{i,0}(t)\n$$\n","which is equivalent to :\n","\n$$\nU'_n - \\frac{c^2}{\\Delta x^2} U_{n-1}(t) + 2c^2(\\frac{1}{\\Delta x^2} + \\frac{1}{\\Delta y^2}) U_n(t) - \\frac{c^2}{\\Delta x^2} U_{n+1}(t) - \\frac{2c^2}{\\Delta y^2} U_{n+I+1}(t) = S_n(t) + \\frac{2c^2}{\\Delta y} K_n(t)\n$$\n","We deduce the matrix $A$ and the vector $F$ as follows:\n","\n$$\n\\begin{cases}\n\\begin{align}\nA_{n,n-1} &= A_{n,n+1} = -\\frac{c^2}{\\Delta x^2} \\\\\nA_{n,n} &= 2c^2 (\\frac{1}{\\Delta x^2} + \\frac{1}{\\Delta y^2}) \\\\\nA_{n,n+I+1} &= -\\frac{2c^2}{\\Delta y^2} \\\\\nF_n(t) &= S_n(t) + \\frac{2c^2}{\\Delta y} K_n(t)\n\\end{align}\n\\end{cases}\n$$\n","## At left edge\n\n","At the left edge, indices $i=0$ and $j$ vary in $[\\![1;J-1]\\!]$.\n","By expanding and summing, the discretization can be written as :\n","\n$$\nu''_{0,j}(t) - \\frac{c^2}{\\Delta y^2} u_{0,j-1}(t) - \\frac{2c^2}{\\Delta x^2} u_{1,j}(t) + 2c^2(\\frac{1}{\\Delta x^2} + \\frac{1}{\\Delta y^2} u_{0,j})(t) - \\frac{c^2}{\\Delta y^2} u_{0,j+1}(t) = s_{0,j}(t) + \\frac{2c^2}{\\Delta x} k_{0,j}(t)\n$$\n","which is equivalent to :\n","\n$$\nU''_n(t) - \\frac{c^2}{\\Delta y^2} U_{n-I-1}(t) - \\frac{2c^2}{\\Delta x^2} U_{n+1}(t) + 2c^2(\\frac{1}{\\Delta x^2} + \\frac{1}{\\Delta y^2}) U_n(t) - \\frac{c^2}{\\Delta y^2} U_{n+I+1}(t) = S_n(t) + \\frac{2c^2}{\\Delta x} K_n(t)\n$$\n","We deduce the matrix $A$ and the vector $F$ as follows:\n","\n$$\n\\begin{cases}\n\\begin{align}\nA_{n, n-I-1} &= A_{n,n+I+1} = -\\frac{c^2}{\\Delta y^2} \\\\\nA_{n,n} &= 2c^2 (\\frac{1}{\\Delta x^2} + \\frac{1}{\\Delta y^2}) \\\\\nA_{n,n+1} &= -\\frac{2c^2}{\\Delta x^2} \\\\\nF_n(t) &= S_n(t) + \\frac{2c^2}{\\Delta x} K_n(t)\n\\end{align}\n\\end{cases}\n$$\n","## At top edge\n\n","At the top edge, indices $i$ vary in $[\\![1;I-1]\\!]$ and $j=J$.\n","By expanding and summing, the discretization can be written as :\n","\n$$\nu''_{i,J}(t) - \\frac{c^2}{\\Delta x^2} u_{i-1,J}(t) + 2c^2(\\frac{1}{\\Delta x^2} + \\frac{1}{\\Delta y^2} u_{i,J})(t) - \\frac{c^2}{\\Delta x^2} u_{i+1,J}(t) - \\frac{2c^2}{\\Delta y^2} u_{i,J-1}(t) = s_{i,J}(t) + \\frac{2c^2}{\\Delta y} k_{i,J}(t)\n$$\n","which is equivalent to :\n","\n$$\nU'_n - \\frac{c^2}{\\Delta x^2} U_{n-1}(t) + 2c^2(\\frac{1}{\\Delta x^2} + \\frac{1}{\\Delta y^2}) U_n(t) - \\frac{c^2}{\\Delta x^2} U_{n+1}(t) - \\frac{2c^2}{\\Delta y^2} U_{n-I-1}(t) = S_n(t) + \\frac{2c^2}{\\Delta y} K_n(t)\n$$\n","We deduce the matrix $A$ and the vector $F$ as follows:\n","\n$$\n\\begin{cases}\n\\begin{align}\nA_{n,n-1} &= A_{n,n+1} = -\\frac{c^2}{\\Delta x^2} \\\\\nA_{n,n} &= 2c^2 (\\frac{1}{\\Delta x^2} + \\frac{1}{\\Delta y^2}) \\\\\nA_{n,n-I-1} &= -\\frac{2c^2}{\\Delta y^2} \\\\\nF_n(t) &= S_n(t) + \\frac{2c^2}{\\Delta y} K_n(t)\n\\end{align}\n\\end{cases}\n$$\n","## At right edge\n\n","At the right edge, indices $i=I$ and $j$ vary in $[\\![1;J-1]\\!]$.\n","By expanding and summing, the discretization can be written as :\n","\n$$\nu''_{I,j}(t) - \\frac{2c^2}{\\Delta x^2} u_{I-1,j}(t) + 2c^2(\\frac{1}{\\Delta x^2} + \\frac{1}{\\Delta y^2} u_{I,j})(t) - \\frac{c^2}{\\Delta y^2} u_{I,j-1}(t) - \\frac{c^2}{\\Delta y^2} u_{I,j+1}(t) = s_{I,j}(t) + \\frac{2c^2}{\\Delta x} k_{I,j}(t)\n$$\n","which is equivalent to :\n","\n$$\nU''_n(t) - \\frac{2c^2}{\\Delta x^2} U_{n-1}(t) + 2c^2(\\frac{1}{\\Delta x^2} + \\frac{1}{\\Delta y^2}) U_n(t) - \\frac{c^2}{\\Delta y^2} U_{n-I-1}(t) - \\frac{c^2}{\\Delta y^2} U_{n+I+1}(t) = S_n(t) + \\frac{2c^2}{\\Delta x} K_n(t)\n$$\n","We deduce the matrix $A$ and the vector $F$ as follows:\n","\n$$\n\\begin{cases}\n\\begin{align}\nA_{n,n-I-1} &= A_{n,n+I+1} = -\\frac{c^2}{\\Delta y^2} \\\\\nA_{n,n-1} &= -\\frac{2c^2}{\\Delta x^2} \\\\\nA_{n,n} &= 2c^2 (\\frac{1}{\\Delta x^2} + \\frac{1}{\\Delta y^2}) \\\\\nF_n(t) &= S_n(t) + \\frac{2c^2}{\\Delta x} K_n(t)\n\\end{align}\n\\end{cases}\n$$\n","## At corners\n\n","At the corners, we do not use virtual points. We approximate the\n","first-order partial derivatives using two-point off-centered differences.\n","## At bottom-left corner\n\n","At the bottom-left corner, indices $i=0$ and $j=0$.\n","By expanding and summing, the discretization can be written as :\n","\n$$\n-\\frac{\\sqrt{2}}{2 \\Delta x} u_{1,0}(t) + (\\frac{\\sqrt{2}}{2 \\Delta x} + \\frac{\\sqrt{2}}{2 \\Delta y}) u_{0,0}(t) - \\frac{\\sqrt{2}}{2 \\Delta y} u_{0,1}(t) = k_{0,0}(t)\n$$\n","which is equivalent to :\n","\n$$\n-\\frac{\\sqrt{2}}{2 \\Delta x} U_{n+1}(t) + (\\frac{\\sqrt{2}}{2 \\Delta x} + \\frac{\\sqrt{2}}{2 \\Delta y}) U_n(t) - \\frac{\\sqrt{2}}{2 \\Delta y} U_{n+I+1}(t) = K_n(t)\n$$\n","We deduce the matrix $A$ and the vector $F$ as follows:\n","\n$$\n\\begin{cases}\n\\begin{align}\nA_{n,n+1} &= -\\frac{\\sqrt{2}}{2 \\Delta x} \\\\\nA_{n,n} &= \\frac{\\sqrt{2}}{2 \\Delta x} + \\frac{\\sqrt{2}}{2 \\Delta y} \\\\\nA_{n,n+I+1} &= -\\frac{\\sqrt{2}}{2 \\Delta y} \\\\\nF_n(t) &= K_n(t)\n\\end{align}\n\\end{cases}\n$$\n","## At top-left corner\n\n","At the top-left corner, indices $i=0$ and $j=J$.\n","By expanding and summing, the discretization can be written as :\n","\n$$\n-\\frac{\\sqrt{2}}{2 \\Delta x} u_{1,J}(t) + (\\frac{\\sqrt{2}}{2 \\Delta x} + \\frac{\\sqrt{2}}{2 \\Delta y}) u_{0,J}(t) - \\frac{\\sqrt{2}}{2 \\Delta y} u_{0,J-1}(t) = k_{0,J}(t)\n$$\n","which is equivalent to :\n","\n$$\n-\\frac{\\sqrt{2}}{2 \\Delta x} U_{n+1}(t) + (\\frac{\\sqrt{2}}{2 \\Delta x} + \\frac{\\sqrt{2}}{2 \\Delta y}) U_n(t) - \\frac{\\sqrt{2}}{2 \\Delta y} U_{n-I-1}(t) = K_n(t)\n$$\n","We deduce the matrix $A$ and the vector $F$ as follows:\n","\n$$\n\\begin{cases}\n\\begin{align}\nA_{n,n+1} &= -\\frac{\\sqrt{2}}{2 \\Delta x} \\\\\nA_{n,n} &= \\frac{\\sqrt{2}}{2 \\Delta x} + \\frac{\\sqrt{2}}{2 \\Delta y} \\\\\nA_{n,n-I-1} &= -\\frac{\\sqrt{2}}{2 \\Delta y} \\\\\nF_n(t) &= K_n(t)\n\\end{align}\n\\end{cases}\n$$\n","## At top-right corner\n\n","At the top-right corner, indices $i=I$ and $j=J$.\n","By expanding and summing, the discretization can be written as :\n","\n$$\n-\\frac{\\sqrt{2}}{2 \\Delta x} u_{I-1,J}(t) + (\\frac{\\sqrt{2}}{2 \\Delta x} + \\frac{\\sqrt{2}}{2 \\Delta y}) u_{I,J}(t) - \\frac{\\sqrt{2}}{2 \\Delta y} u_{I,J-1}(t) = k_{I,J}(t)\n$$\n","which is equivalent to :\n","\n$$\n-\\frac{\\sqrt{2}}{2 \\Delta x} U_{n-1}(t) + (\\frac{\\sqrt{2}}{2 \\Delta x} + \\frac{\\sqrt{2}}{2 \\Delta y}) U_n(t) - \\frac{\\sqrt{2}}{2 \\Delta y} U_{n-I-1}(t) = K_n(t)\n$$\n","We deduce the matrix $A$ and the vector $F$ as follows:\n","\n$$\n\\begin{cases}\n\\begin{align}\nA_{n,n-1} &= -\\frac{\\sqrt{2}}{2 \\Delta x} \\\\\nA_{n,n} &= \\frac{\\sqrt{2}}{2 \\Delta x} + \\frac{\\sqrt{2}}{2 \\Delta y} \\\\\nA_{n,n-I-1} &= -\\frac{\\sqrt{2}}{2 \\Delta y} \\\\\nF_n(t) &= K_n(t)\n\\end{align}\n\\end{cases}\n$$\n","## At bottom-right corner\n\n","At the bottom-right corner, indices $i=I$ and $j=0$.\n","By expanding and summing, the discretization can be written as :\n","\n$$\n-\\frac{\\sqrt{2}}{2 \\Delta x} u_{I-1,0}(t) + (\\frac{\\sqrt{2}}{2 \\Delta x} + \\frac{\\sqrt{2}}{2 \\Delta y}) u_{I,0}(t) - \\frac{\\sqrt{2}}{2 \\Delta y} u_{I,1}(t) = k_{I,0}(t)\n$$\n","which is equivalent to :\n","\n$$\n-\\frac{\\sqrt{2}}{2 \\Delta x} U_{n-1}(t) + (\\frac{\\sqrt{2}}{2 \\Delta x} + \\frac{\\sqrt{2}}{2 \\Delta y}) U_n(t) - \\frac{\\sqrt{2}}{2 \\Delta y} U_{n+I+1}(t) = K_n(t)\n$$\n","We deduce the matrix $A$ and the vector $F$ as follows:\n","\n$$\n\\begin{cases}\n\\begin{align}\nA_{n,n-1} &= -\\frac{\\sqrt{2}}{2 \\Delta x} \\\\\nA_{n,n} &= \\frac{\\sqrt{2}}{2 \\Delta x} + \\frac{\\sqrt{2}}{2 \\Delta y} \\\\\nA_{n,n+I+1} &= -\\frac{\\sqrt{2}}{2 \\Delta y} \\\\\nF_n(t) &= K_n(t)\n\\end{align}\n\\end{cases}\n$$\n","## Time discretization\n\n","After discretization and elimination, the semi-discretized wave equation in space can be written in the form :\n","\n$$\n\\begin{cases}\n\\begin{align}\n\\tilde U''(t) + A \\tilde U(t) &= F(t) \\\\\n\\tilde U(0) &= \\tilde U^0 \\\\\n\\tilde U'(0) &= V^0\n\\end{align}\n\\end{cases}\n$$\n","By approximating the second-order time derivative with a three-point\n","central difference, we obtain a relation between\n","$\\tilde U^{n+1}$, $\\tilde U^n$ and $\\tilde U^{n-1}$ as follows:\n","\n$$\n\\frac{\\tilde U^{n+1} - 2 \\tilde U^n + \\tilde U^{n-1}}{\\Delta t^2} + A \\tilde U^n = F^n\n$$\n","Consequently, we obtain the following explicit scheme :\n","\n$$\n\\tilde U^{n+1} = 2 \\tilde U^n - \\tilde U^{n-1} + \\Delta t^2 (F^n - A \\tilde U^n)\n$$\n","Initializing this scheme requires the values of $\\tilde U^0 = \\tilde U(0)$ and $\\tilde U^1 \\approx \\tilde U(\\Delta t)$.\n","Using $\\tilde U(\\Delta t) \\approx \\tilde U(0) + \\Delta t \\tilde U'(0) + \\frac{\\Delta t^2}{2} \\tilde U''(0)$, we rewrite the scheme in the following form :\n","\n$$\n\\begin{cases}\n\\begin{align}\n\\tilde U^0_k &= U^0_k = f(x_i,y_j) \\quad \\text{with } k=i+j(I+1) \\\\\n\\tilde U^1 &= \\tilde U^0 + \\Delta t V^0 + \\frac{\\Delta t^2}{2} (F^0 - A \\tilde U^0) \\quad \\text{with } V^0_k = g(x_i,y_j)\n\\end{align}\n\\end{cases}\n$$\n","## Implementation\n\n"],"metadata":{}},{"cell_type":"code","execution_count":0,"metadata":{"slideshow":{"slide_type":"fragment"}},"outputs":[],"source":["from feelpp_sonorhc.fd import wave_2d\n","import numpy as np\n","\n","L, nx = 2., 100\n","H, ny = 2., 100\n","T = 4.\n","c = 4. # m/s\n","\n","# source term\n","def s(x: np.ndarray, y: np.ndarray, t: float) -> np.ndarray:\n","    return np.zeros_like(x)\n","\n","# neumann condition\n","def k(x: np.ndarray, y: np.ndarray, t: float) -> np.ndarray:\n","    return np.zeros_like(x)\n","\n","# gaussian function\n","def gaussian(x: np.ndarray, y: np.ndarray, A: float, sigma: float, x0: float, y0: float) -> np.ndarray:\n","    return A * np.exp(-((x - x0)**2 + (y - y0)**2) / (2 * sigma**2))\n","\n","# initial condition 1\n","def f(x: np.ndarray, y: np.ndarray) -> np.ndarray:\n","    return gaussian(x, y, A=0.3, sigma=0.05, x0=1., y0=1.)\n","\n","# initial condition 2\n","def g(x: np.ndarray, y: np.ndarray) -> np.ndarray:\n","    return np.zeros_like(x)\n","\n","# solve the problem\n","U = wave_2d.solve_wave2D_fdtd(c, s, f, g, k, L, nx, H, ny, T)\n","print(U.shape)\n"]},{"cell_type":"markdown","source":["## Visualization\n\n","We use the library pyvista to visualize the solution.\n"],"metadata":{}},{"cell_type":"code","execution_count":0,"metadata":{"slideshow":{"slide_type":"fragment"}},"outputs":[],"source":["import pyvista as pv\n","from IPython.display import Image, display\n","\n","multi_block = pv.MultiBlock()\n","x = np.linspace(0, L, nx + 1)\n","y = np.linspace(0, H, ny + 1)\n","x, y = np.meshgrid(x, y)\n","z = np.zeros_like(x)\n","\n","for i in range(U.shape[1]):\n","    z = U[:, i].reshape(nx + 1, ny + 1)\n","    grid = pv.StructuredGrid(x, y, z)\n","    grid[\"Amplitude\"] = z.ravel()\n","    multi_block[f\"Time_{i}\"] = grid\n","\n","plotter = pv.Plotter()\n","plotter.open_gif(\"wave_animation.gif\")\n","\n","T_iter = len(multi_block_3D)\n","min_value = np.min(U)\n","max_value = np.max(U)\n","\n","for i in range(len(multi_block_3D)):\n","    plotter.clear()\n","    block = multi_block_3D[i]\n","    plotter.add_mesh(block, cmap=\"coolwarm\", show_edges=False, clim=(min_value, max_value))\n","    plotter.view_isometric()\n","    plotter.add_axes()\n","    plotter.add_text(f\"Elapsed time: {(T * i) / T_iter:.2f} s\", position='upper_left', font_size=10, color='black')\n","    plotter.write_frame()\n","plotter.close()\n","\n","display(Image(filename=\"wave_animation.gif\"))\n"]}],"metadata":{"language_info":{"name":"python","version":"3.9.1"}},"nbformat":4,"nbformat_minor":4}